more rules

theories/iris/language/lwp_resources.v
@@ -34,4 +34,52 @@ Locate Wasm.iris.language.iris.iris.val.
       iFrame.
   Qed.
 
+  Check wp_set_local.
+
+  Definition lp_fr_set f i v (Φ : @logpred Σ) : logpred :=
+    {|
+      lp_fr := λ f', ⌜f' = {| f_locs := seq.set_nth v (f_locs f) i v; f_inst := f_inst f |}⌝;
+      lp_val := lp_val Φ;
+      lp_trap := lp_trap Φ;
+      lp_br := lp_br Φ;
+      lp_ret := lp_ret Φ;
+      lp_host := lp_host Φ;
+    |}.
+
+  Definition lp_run Φ :=
+    {|
+      lp_fr := lp_fr Φ;
+      lp_val := λ vs, lp_val Φ vs ∗ ↪[RUN];
+      lp_trap := lp_trap Φ;
+      lp_br := λ x, lp_br Φ x ∗ ↪[RUN];
+      lp_ret := λ x, lp_ret Φ x ∗ ↪[RUN];
+      lp_host := λ ft hf vs lh, lp_host Φ ft hf vs lh ∗ ↪[RUN];
+    |}.
+
+  Lemma lp_run_sep Φ w :
+    denote_logpred Φ w ∗ ↪[RUN] ⊢ denote_logpred (lp_run Φ) w.
+  Proof.
+    unfold lp_run, denote_logpred.
+    cbn.
+    destruct w; cbn; iIntros "[HΦ Hrun]"; iFrame.
+  Qed.
+
+  Lemma lenient_wp_set_local s E i Φ v (f: datatypes.frame) :
+    i < length f.(f_locs) ->
+    ▷ Φ.(lp_val) [] ∗
+    ↪[frame] f ∗
+    ↪[RUN]
+    ⊢ lenient_wp s E [AI_basic (BI_const v); AI_basic (BI_set_local i)] (lp_run (lp_fr_set f i v Φ)).
+  Proof.
+    iIntros (Hlen) "(Hval & Hf & Hrun)".
+    iApply (wp_wand with "[Hval Hf Hrun]").
+    iApply (wp_set_local with "[Hval] [$Hf] [$Hrun]").
+    - assumption.
+    - instantiate (1:= lp_noframe (lp_fr_set f i v Φ)).
+      by cbn.
+    - iIntros (w) "((Hpred & Hrun) & Hf)".
+      iApply lp_run_sep.
+      by iFrame.
+  Qed.
+
 End lwp_resources.
